Util/Vector/VecArith.v
@@ -1,0 +1,101 @@
+(**
+CoLoR, a Coq library on rewriting and termination.
+See the COPYRIGHTS and LICENSE files.
+
+- Adam Koprowski, 2007-04-02
+
+Arithmetic over vectors of natural numbers.
+*)
+
+Set Implicit Arguments.
+
+Require Export VecUtil.
+Require Export RelUtil.
+
+Section VecArith.
+
+Variables n : nat.
+
+Notation vec := (vector nat).
+Notation vecn := (vec n).
+
+(***********************************************************************)
+(** [ge] on vectors *)
+
+Definition vec_ge := Vforall2n ge.
+Infix ">=v" := vec_ge (at level 70).
+
+Lemma vec_tail_ge : forall n (v v' : vec (S n)), v >=v v' -> Vtail v >=v Vtail v'.
+
+Proof.
+  unfold vec_ge. intros.
+  apply Vforall2_intro. intros.
+  do 2 rewrite Vnth_tail.
+  apply (Vforall2_nth ge). assumption.
+Qed.
+
+Lemma vec_ge_dec : rel_dec (@vec_ge n).
+
+Proof.
+  intros P Q. destruct (Vforall2_dec nat_ge_dec P Q); intuition.
+Defined.
+
+Lemma vec_ge_refl : reflexive (@vec_ge n).
+
+Proof.
+  intros x. unfold vec_ge. apply Vforall2_intro. intros.
+  unfold ge. apply le_refl.
+Qed.
+
+Lemma vec_ge_trans : transitive (@vec_ge n).
+
+Proof.
+  intros x y z xy yz. unfold vec_ge.
+  apply Vforall2_intro. intros.
+  unfold ge. apply le_trans with (Vnth y ip).
+  apply (Vforall2_nth ge). assumption.
+  apply (Vforall2_nth ge). assumption.
+Qed.
+
+(***********************************************************************)
+(** vector plus *)
+
+Definition zero_vec := Vconst 0 n.
+
+Definition vector_plus (v1 v2 : vecn) := Vmap2 plus v1 v2.
+Infix "[+]" := vector_plus (at level 50).
+
+Definition add_vectors i (v : vector vecn i) := Vfold_left vector_plus zero_vec v.
+
+(***********************************************************************)
+(** compatibility of [vec_plus] with [vec_ge] *)
+
+Lemma vec_plus_ge_compat : forall vl vl' vr vr', vl >=v vl' -> vr >=v vr' -> vl [+] vr >=v vl' [+] vr'.
+
+Proof.
+  unfold vector_plus, vec_ge. intros. apply Vforall2_intro.
+  intros. simpl. do 2 rewrite Vmap2_nth.
+  unfold ge. apply plus_le_compat.
+  apply (Vforall2_nth ge). assumption.
+  apply (Vforall2_nth ge). assumption.
+Qed.
+
+Lemma vec_plus_ge_compat_r : forall vl vl' vr, vl >=v vl' -> vl [+] vr >=v vl' [+] vr.
+
+Proof.
+  intros. apply vec_plus_ge_compat. assumption. exact (vec_ge_refl vr).
+Qed.
+
+Lemma vec_plus_ge_compat_l : forall vl vr vr', vr >=v vr' -> vl [+] vr >=v vl [+] vr'.
+  
+Proof.
+  intros. apply vec_plus_ge_compat. exact (vec_ge_refl vl). assumption.
+Qed.
+ 
+End VecArith.
+
+(***********************************************************************)
+(** Notations *)
+
+Infix ">=v" := vec_ge (at level 70).
+Infix "[+]" := vector_plus (at level 50).
